src/Verification.v
@@ -9,19 +9,79 @@ Import ListNotations.
 Require Import PeanoNat.
 Import Nat.
 Module Verification.
-Inductive compile : Language.state -> Assembly.state -> Prop :=
-  | comp_r : forall p a, Compiler.compile p = Some a -> compile p a.
-
 Definition eval := Language.semantics.
 Definition eval' := Assembly.semantics.
-
+Theorem comp_newstate :
+  forall p q, Compiler.compile p q ->
+              q.(Assembly.pc) = Compiler.new_pc (p.(Language.prog)) (p.(Language.pc)) /\
+              q.(Assembly.ac) = p.(Language.ptr) /\
+              q.(Assembly.mem) = p.(Language.mem) /\
+              q.(Assembly.b) = 0.
+Proof.
+Admitted.
+Theorem match_preserve : 
+  forall p p', Language.semantics p p' ->
+               Compiler.matched (Language.prog p) ->
+               Compiler.matched (Language.prog p').
+Proof.
+Admitted.
+Theorem ptrinc_comp :
+  forall p q, Compiler.compile p q -> 
+              Language.read_instr p Language.PtrInc ->
+              Assembly.read_instr q (Assembly.Add 1).
+Proof.
+Admitted.
+Theorem ptrdec_comp :
+  forall p q, Compiler.compile p q -> 
+              Language.read_instr p Language.PtrDec ->
+              Assembly.read_instr q (Assembly.Sub 1).
+Proof.
+Admitted.
+Theorem inc_comp :
+  forall p q, Compiler.compile p q -> 
+              Language.read_instr p Language.Inc ->
+              Assembly.read_instr q (Assembly.Swap).
+Proof.
+Admitted.
+Theorem dec_comp :
+  forall p q, Compiler.compile p q -> 
+              Language.read_instr p Language.Dec ->
+              Assembly.read_instr q (Assembly.Swap).
+Proof.
+Admitted.
+Theorem jump_comp :
+  forall p q, Compiler.compile p q -> 
+              Language.read_instr p Language.Jump ->
+              Assembly.read_instr q (Assembly.Skip).
+Proof.
+Admitted.
+Theorem ret_comp :
+  forall p q, Compiler.compile p q -> 
+              Language.read_instr p Language.Ret ->
+              Assembly.read_instr q (Assembly.Skip).
+Proof.
+Admitted.
 Theorem comp_correct : 
-  Simulation.plus_forward_sim compile eval eval'.
+  Simulation.plus_forward_sim Compiler.compile eval eval'.
 Proof.
   unfold Simulation.plus_forward_sim.
-  induction p.
+  intros p q compileH p' evalH.
+  assert (Compiler.matched (Language.prog p')).
+  apply match_preserve with (p := p).
+  unfold eval in evalH.
+  assumption.
+  inversion compileH.
+  assumption.
+  induction evalH.
+  - exists (Compiler.compile' p').
+    split.
+    + apply Compiler.comp_r.
+      assumption.
+      reflexivity.
+    + inversion compileH.
+      remember (Compiler.compile' p') as q'.
+      assert (Assembly.read_instr q (Assembly.Add 1)).
 
-    
 Admitted. (* to be done. *)
 
 End Verification.
